Added various ways of configuring the parser.

Expressions.thy
@@ -1,15 +1,25 @@
 theory Expressions
   imports Variables
+  keywords "pretty_exprs" "full_exprs" "lit_vars" "expr_vars" "expr_ctr" :: "thy_decl_block"
 begin
 
 named_theorems expr_defs
 
+text \<open> An expression is represented simply as a function from the state space @{typ "'s"} to
+  the return type @{typ "'a"}, which is the simplest shallow model for Isabelle/HOL. 
+
+  The aim of this theory is to provide transparent conversion between this representation 
+  and a more intuitive expression syntax. For example, an expression @{term "x + y"} where 
+  $x$ and $y$ are both state variables, can be represented by @{term "\<lambda> s. get\<^bsub>x\<^esub> s + get\<^bsub>y\<^esub> s"} 
+  when both variables are modelled using lenses. Rather than having to write $\lambda$-terms 
+  directly, it is more convenient to hide this threading of state behind a parser. \<close>
+
 type_synonym ('a, 's) expr = "'s \<Rightarrow> 'a"
 
-definition SEXP :: "('s \<Rightarrow> 'a) \<Rightarrow> ('a, 's) expr" ("[_]\<^sub>E") where
+definition SEXP :: "('s \<Rightarrow> 'a) \<Rightarrow> ('a, 's) expr" ("[_]\<^sub>e") where
 [expr_defs]: "SEXP x = x"
 
-lemma SEXP_idem [simp]: "[[e]\<^sub>E]\<^sub>E = [e]\<^sub>E" by (simp add: SEXP_def)
+lemma SEXP_idem [simp]: "[[e]\<^sub>e]\<^sub>e = [e]\<^sub>e" by (simp add: SEXP_def)
 
 abbreviation (input) var :: "('a \<Longrightarrow> 's) \<Rightarrow> ('a, 's) expr" where
 "var x \<equiv> (\<lambda> s. get\<^bsub>x\<^esub> s)"
@@ -21,32 +31,74 @@ abbreviation (input) bop
   :: "('a \<Rightarrow> 'b \<Rightarrow> 'c) \<Rightarrow> ('a, 's) expr \<Rightarrow> ('b, 's) expr \<Rightarrow> ('c, 's) expr" where
 "bop f e\<^sub>1 e\<^sub>2 \<equiv> (\<lambda> s. f (e\<^sub>1 s) (e\<^sub>2 s))"
 
+nonterminal sexp
+
 syntax
   "_sexp_state" :: "id"
-  "_sexp_quote" :: "logic \<Rightarrow> logic" ("U'(_')")
+  "_sexp_quote" :: "logic \<Rightarrow> logic" ("'(_')\<^sub>e")
   "_sexp_lit"   :: "logic \<Rightarrow> logic" ("\<guillemotleft>_\<guillemotright>")
   "_sexp_var"   :: "svid \<Rightarrow> logic" ("&_" [990] 990)
-  "_sexp_evar"  :: "id \<Rightarrow> logic" ("@_" [999] 999)
+  "_sexp_evar"  :: "id_position \<Rightarrow> logic" ("@_" [999] 999)
+  "_sexp_pqt"   :: "logic \<Rightarrow> sexp" ("[_]\<^sub>e")
+
+
+ML \<open>
+val state_id = "\<s>";
+\<close>
 
 parse_translation \<open> 
-  [(@{syntax_const "_sexp_state"}, fn ctx => fn term => Syntax.free "STATE")]
+  [(@{syntax_const "_sexp_state"}, fn ctx => fn term => Syntax.free state_id)]
 \<close>
 
 translations
-  "_sexp_lit x" => "x"
+(*  "_sexp_lit x" => "x" *)
   "_sexp_var x" => "get\<^bsub>x\<^esub> _sexp_state"
-  "_sexp_evar e" => "e _sexp_state"
+(*  "_sexp_evar e" => "e _sexp_state" *)
 
 ML \<open>
+structure LitVars = Theory_Data
+  (type T = bool
+   val empty = false
+   val extend = I
+   val merge = (fn (x, y) => x orelse y));
+
+Outer_Syntax.command @{command_keyword "lit_vars"} "treat variables as literals by default" 
+  (Scan.succeed (Toplevel.theory (LitVars.put true)));
+
+Outer_Syntax.command @{command_keyword "expr_vars"} "treat variables as expressions by default" 
+  (Scan.succeed (Toplevel.theory (LitVars.put false)));
+
+structure FullExprs = Theory_Data
+  (type T = bool
+   val empty = false
+   val extend = I
+   val merge = (fn (x, y) => x orelse y));
+
+Outer_Syntax.command @{command_keyword "full_exprs"} "print full form of expressions" 
+  (Scan.succeed (Toplevel.theory (FullExprs.put true)));
+
+Outer_Syntax.command @{command_keyword "pretty_exprs"} "pretty print expressions" 
+  (Scan.succeed (Toplevel.theory (FullExprs.put false)));
+
 structure NoLift = Theory_Data
   (type T = unit Symtab.table
    val empty = Symtab.empty
    val extend = I
    val merge = Symtab.merge (K true));
 
-fun nolift_const n thy =  
+fun nolift_const thy n =  
           let val Const (c, _) = Proof_Context.read_const {proper = true, strict = false} (Proof_Context.init_global thy) n 
-          in NoLift.map (Symtab.update (c, ())) thy end
+          in NoLift.map (Symtab.update (c, ())) thy end;
+
+Outer_Syntax.command @{command_keyword "expr_ctr"} "declare that certain constants should not be lifted"
+    (Scan.repeat1 (Parse.term)
+     >> (fn ns => 
+         Toplevel.theory 
+         (fn thy => Library.foldl (fn (thy, n) => nolift_const thy n) (thy, ns))));
+
+
+Outer_Syntax.command @{command_keyword "full_exprs"} "print full form of expressions" 
+
 \<close>
 
 ML \<open> 
@@ -57,12 +109,16 @@ fun lift_expr_aux ctx (Const (n', t), args) =
     val args' = map (lift_expr ctx) args
   in if (n = @{const_name lens_get} orelse n = @{const_name SEXP}) 
      then Term.list_comb (Const (n', t), args)
+     else if (n = @{syntax_const "_sexp_lit"})
+     then Term.list_comb (hd args, tl args')
+     else if (n = @{syntax_const "_sexp_evar"})
+     then Term.list_comb (hd args $ free state_id, tl args')
      else if (member (op =) (Symtab.keys (NoLift.get (Proof_Context.theory_of ctx))) n)
-     then Term.list_comb (Const (n', t), args) $ free "STATE"
+     then Term.list_comb (Const (n', t), args) $ free state_id
      else
      case (Type_Infer_Context.const_type ctx n) of
       SOME (Type (\<^type_name>\<open>lens_ext\<close>, _)) 
-        => Term.list_comb (const @{const_name lens_get} $ Const (n', t) $ free "STATE", args') |
+        => Term.list_comb (const @{const_name lens_get} $ Const (n', t) $ free state_id, args') |
       _ => Term.list_comb (Const (n, t), args')
   end |
 lift_expr_aux ctx (Free (n, t), args) = 
@@ -75,60 +131,95 @@ lift_expr_aux ctx (Free (n, t), args) =
           lift_expr_aux ctx (Const (c, t), args)
         \<comment> \<open> Otherwise, we leave it alone \<close>
         else
-          Term.list_comb (Free (n, t), args)
+          let val trm = if (LitVars.get (Proof_Context.theory_of ctx)) 
+                        then Free (n, t) else Free (n, t) $ Syntax.free state_id
+          in Term.list_comb (trm, map (lift_expr ctx) args) end
   end |
 lift_expr_aux ctx (e, args) = Term.list_comb (e, args)
 and 
 lift_expr ctx (Abs (n, t, e)) = 
-  if (n = "STATE") then Abs (n, t, e) else Abs (n, t, lift_expr ctx e) |
-lift_expr ctx e = lift_expr_aux ctx (Term.strip_comb e)
-
-(*
-fun
-  (* FIXME: Add a command to allow certain constants to be ignored and their parameters not interpreted. *)
-  lift_expr _ (Const (@{const_syntax lens_get}, t) $ x) = (Const (@{const_name lens_get}, t) $ x) |
-  lift_expr _ (Const (@{const_syntax lens_get}, t) $ x $ y) = (Const (@{const_name lens_get}, t) $ x $ y) |
-  lift_expr ctx (Const (n', t)) =
-  let val n = (if (Lexicon.is_marked n') then Lexicon.unmark_const n' else n')
-  in case (Type_Infer_Context.const_type ctx n) of
-      SOME (Type (\<^type_name>\<open>lens_ext\<close>, _)) => Const (@{const_name lens_get}, dummyT) $ Const (n', t) $ Syntax.free "STATE" |
-      _ => Const (n, t)
-  end |
-lift_expr ctx (Free (n, t)) = 
-    let val consts = (Proof_Context.consts_of ctx)
-        val {const_space, ...} = Consts.dest consts
-        \<comment> \<open> The name must be internalised in case it needs qualifying. \<close>
-        val c = Consts.intern consts n in
-        \<comment> \<open> If the name refers to a declared constant, then we lift it as a constant. \<close>
-        if (Name_Space.declared const_space c) then
-          lift_expr ctx (Const (c, t))
-        \<comment> \<open> Otherwise, we leave it alone \<close>
-        else
-          Free (n, t)
-  end |
-lift_expr ctx (f $ x) = lift_expr ctx f $ lift_expr ctx x |
-lift_expr _ x = x 
-*)
+  if (n = state_id) then Abs (n, t, e) else Abs (n, t, lift_expr ctx e) |
+lift_expr ctx e = lift_expr_aux ctx ((Term.strip_comb e))
 \<close>
 
 parse_translation \<open>
   [(@{syntax_const "_sexp_quote"}
-   , fn ctx => fn term => 
-      Syntax.const @{const_name SEXP} 
-      $ (lambda (Syntax.free "STATE") (lift_expr ctx (hd term))))]
+   , fn ctx => fn terms =>
+      case terms of
+        [Const (@{const_syntax SEXP}, t) $ e] => Const (@{const_name SEXP}, t) $ e |
+        [e] =>
+            Syntax.const @{const_name SEXP} 
+            $ (lambda (Syntax.free state_id) (lift_expr ctx (Term_Position.strip_positions e))))]
 \<close>
+
+ML \<open> \<close>
+
+ML \<open> 
+tl;
+
+fun print_expr_aux ctx (f, args) =
+  let open Proof_Context
+      fun sexp_evar x = if (LitVars.get (theory_of ctx)) then Syntax.const "_sexp_evar" $ x else x
+  in
+  case (f, args) of
+    (Const (@{syntax_const "_free"}, _), (Free (n, t) :: Const (@{syntax_const "_sexp_state"}, _) :: r)) => 
+     sexp_evar (Term.list_comb (Syntax.const @{syntax_const "_free"} $ Free (n, t)
+                              , map (print_expr ctx) r)) |
+    (Const (@{const_syntax lens_get}, _), [x, Const (@{syntax_const "_sexp_state"}, _)])
+      => Syntax.const @{syntax_const "_sexp_var"} $ x |
+    (Free (n, t), [Const (@{syntax_const "_sexp_state"}, _)]) 
+      => sexp_evar (Free (n, t)) | 
+    _ => if (length args > 0)
+         then case (List.last args) of
+           Const (@{syntax_const "_sexp_state"}, _) => 
+             Term.list_comb (f, map (print_expr ctx) (take (length args - 1) args)) |
+           _ => Term.list_comb (f, map (print_expr ctx) args)
+         else Term.list_comb (f, map (print_expr ctx) args)
+   end
+and 
+print_expr ctx (Abs (n, t, e)) = Abs (n, t, print_expr ctx e) |
+print_expr ctx e = print_expr_aux ctx (Term.strip_comb e)
+
+fun strip_sexp_state (f, args) =
+  let val args' = filter (fn x => case x of Const (@{syntax_const "_sexp_state"}, _) => false | _ => true) args
+      val args'' = map (strip_sexp_state o Term.strip_comb) args'
+  in Term.list_comb (f, args'') end;
+\<close>
+
 print_translation \<open>
   [(@{const_syntax "SEXP"}
    , fn ctx => fn ts =>
+     if (FullExprs.get (Proof_Context.theory_of ctx)) 
+     then Syntax.const @{syntax_const "_sexp_pqt"} $ hd ts 
+     else
      Syntax.const @{syntax_const "_sexp_quote"} 
-     $ betapply (hd ts, Syntax.const @{syntax_const "_sexp_state"}))]
+     $ print_expr ctx (betapply ((hd ts), Syntax.const @{syntax_const "_sexp_state"})))]
 \<close>
 
-translations
-  "&x" <= "get\<^bsub>x\<^esub> _sexp_state"
-  "@e" <= "e _sexp_state"
+lit_vars
 
-lemma "U(v \<in> &xs \<union> ys \<union> {} \<and> @e) = undefined"
+term "(f \<s> + \<guillemotleft>x\<guillemotright>)\<^sub>e"
+
+full_exprs
+
+term "(\<guillemotleft>f\<guillemotright> (@e))\<^sub>e"
+
+term "(f)\<^sub>e"
+
+expr_vars
+
+full_exprs
+
+term "SEXP(\<lambda> \<s>. get\<^bsub>x\<^esub> \<s> + e \<s> + v)"
+
+pretty_exprs
+expr_vars
+
+term "(@x)\<^sub>e"
+
+term "SEXP(\<lambda> \<s>. get\<^bsub>x\<^esub> \<s> + e \<s> + v)"
+
+lemma "(v \<in> (&xs) \<union> (&f) ys \<union> {} \<and> @e)\<^sub>e = undefined"
   apply (simp) oops
 
 end
