Shallow_Expressions.thy
@@ -1,5 +1,3 @@
 theory Shallow_Expressions
   imports Variables Expressions Unrestriction Substitutions
-begin
-
-end
+begin end
