Substitutions.thy
@@ -18,7 +18,7 @@ definition subst_upd :: "'s subst \<Rightarrow> ('a \<Longrightarrow> 's) \<Righ
   where [expr_defs]: "subst_upd \<sigma> x e = (\<lambda> s. put\<^bsub>x\<^esub> (\<sigma> s) (e s))"
 
 definition subst_lookup :: "('s\<^sub>1,'s\<^sub>2) psubst \<Rightarrow> ('a \<Longrightarrow> 's\<^sub>2) \<Rightarrow> ('a, 's\<^sub>1) expr" ("\<langle>_\<rangle>\<^sub>s")
-  where [expr_defs]: "\<langle>\<sigma>\<rangle>\<^sub>s = (\<lambda> x b. get\<^bsub>x\<^esub> (\<sigma> b))"
+  where [expr_defs]: "\<langle>\<sigma>\<rangle>\<^sub>s x = (\<lambda> s. get\<^bsub>x\<^esub> (\<sigma> s))"
 
 definition unrest_usubst :: "('a \<Longrightarrow> 's) \<Rightarrow> 's subst \<Rightarrow> bool" 
   where [expr_defs]: "unrest_usubst x \<sigma> = (\<forall> \<rho> v. \<sigma> (put\<^bsub>x\<^esub> \<rho> v) = put\<^bsub>x\<^esub> (\<sigma> \<rho>) v)"
@@ -52,7 +52,7 @@ syntax
     
 translations
   "_SubstUpd m (_SMaplets xy ms)"     == "_SubstUpd (_SubstUpd m xy) ms"
-  "_SubstUpd m (_smaplet x y)"        == "CONST subst_upd m x U(y)"
+  "_SubstUpd m (_smaplet x y)"        == "CONST subst_upd m x (y)\<^sub>e"
 (*  "_SubstUpd m (_smaplet x y)"        <= "CONST subst_upd m x y" *)
   "_Subst ms"                         == "_SubstUpd id\<^sub>s ms"
   "_Subst (_SMaplets ms1 ms2)"        <= "_SubstUpd (_Subst ms1) ms2"
@@ -61,8 +61,8 @@ translations
   "_SMaplets ms1 (_SMaplets ms2 ms3)" <= "_SMaplets (_SMaplets ms1 ms2) ms3"
   "_subst P es vs" => "CONST subst_app (_psubst id\<^sub>s vs es) P"
   "_psubst m (_salphas x xs) (_uexprs v vs)" => "_psubst (_psubst m x v) xs vs"
-  "_psubst m x v"  => "CONST subst_upd m x U(v)"
-  "_subst P v x" <= "CONST subst_app (CONST subst_upd id\<^sub>s x U(v)) P"
+  "_psubst m x v"  => "CONST subst_upd m x (v)\<^sub>e"
+  "_subst P v x" <= "CONST subst_app (CONST subst_upd id\<^sub>s x (v)\<^sub>e) P"
 (*
   "_subst P v x" <= "_subst P (_spvar x) v"
 *)
@@ -73,16 +73,16 @@ subsection \<open> Substitution Laws \<close>
 named_theorems usubst and usubst_eval
 
 lemma subst_unrest [usubst]:
-  "\<lbrakk> vwb_lens x; x \<sharp> @v \<rbrakk> \<Longrightarrow> \<sigma>(x \<mapsto>\<^sub>s @e) \<dagger> v = \<sigma> \<dagger> v"
+  "\<lbrakk> vwb_lens x; x \<sharp> v \<rbrakk> \<Longrightarrow> \<sigma>(x \<mapsto>\<^sub>s e) \<dagger> v = \<sigma> \<dagger> v"
   by (auto simp add: expr_defs fun_eq_iff)
 
 lemma subst_lookup_id [usubst]: "\<langle>id\<^sub>s\<rangle>\<^sub>s x = var x"
   by (simp add: expr_defs)
 
-lemma subst_id_var: "id\<^sub>s = U(&\<^bold>v)"
+lemma subst_id_var: "id\<^sub>s = (&\<^bold>v)\<^sub>e"
   by (simp add: expr_defs lens_defs)
 
-lemma subst_upd_id_lam [usubst]: "subst_upd U(&\<^bold>v) x v = subst_upd id\<^sub>s x v"
+lemma subst_upd_id_lam [usubst]: "subst_upd (&\<^bold>v)\<^sub>e x v = subst_upd id\<^sub>s x v"
   by (simp add: subst_id_var)
 
 lemma subst_id [simp]: "id\<^sub>s \<circ> \<sigma> = \<sigma>" "\<sigma> \<circ> id\<^sub>s = \<sigma>"
@@ -93,35 +93,36 @@ lemma subst_lookup_one_lens [usubst]: "\<langle>\<sigma>\<rangle>\<^sub>s 1\<^su
 
 (* FIXME: Figure out how to make laws like this parse and simplify *)
 
+expr_ctr subst_app
 
-setup \<open> nolift_const @{const_name subst_app} \<close>
-
+(*
 translations 
   "CONST subst_app \<sigma> e" <= "CONST subst_app \<sigma> e _sexp_state"
+*)
 
-term "U(f (\<sigma> \<dagger> @e))"
+term "(f (\<sigma> \<dagger> e))\<^sub>e"
 
-term "U(\<forall> x. x + &y > &z)"
+term "(\<forall> x. x + &y > &z)\<^sub>e"
 
-term "U(\<forall> k. P\<lbrakk>k/x\<rbrakk>)"
+term "(\<forall> k. P\<lbrakk>\<guillemotleft>k\<guillemotright>/x\<rbrakk>)\<^sub>e"
 
-lemma subst_var [usubst]: "\<sigma> \<dagger> U(&x) = \<langle>\<sigma>\<rangle>\<^sub>s x"
+lemma subst_var [usubst]: "\<sigma> \<dagger> (&x)\<^sub>e = \<langle>\<sigma>\<rangle>\<^sub>s x"
   by (simp add: expr_defs)
 
 text \<open> We can't use this as simplification unfortunately as the expression structure is too
   ambiguous to support automatic rewriting. \<close>
 
-lemma subst_uop: "\<sigma> \<dagger> U(f (@e)) = U(f (\<sigma> \<dagger> U(@e)))"
+lemma subst_uop: "\<sigma> \<dagger> (\<guillemotleft>f\<guillemotright> e)\<^sub>e = (\<guillemotleft>f\<guillemotright> (\<sigma> \<dagger> e))\<^sub>e"
   by (simp add: expr_defs)
 
-lemma subst_bop: "\<sigma> \<dagger> U(f (@e\<^sub>1) (@e\<^sub>2)) = U(f (\<sigma> \<dagger> U(@e\<^sub>1)) (\<sigma> \<dagger> U(@e\<^sub>2)))"
+lemma subst_bop: "\<sigma> \<dagger> (\<guillemotleft>f\<guillemotright> e\<^sub>1 e\<^sub>2)\<^sub>e = (\<guillemotleft>f\<guillemotright> (\<sigma> \<dagger> e\<^sub>1) (\<sigma> \<dagger> e\<^sub>2))\<^sub>e"
   by (simp add: expr_defs)
 
 text \<open> A substitution update naturally yields the given expression. \<close>
     
 lemma subst_lookup_upd [usubst]:
   assumes "weak_lens x"
-  shows "\<langle>\<sigma>(x \<mapsto>\<^sub>s v)\<rangle>\<^sub>s x = U(v)"
+  shows "\<langle>\<sigma>(x \<mapsto>\<^sub>s v)\<rangle>\<^sub>s x = (v)\<^sub>e"
   using assms by (simp add: expr_defs)
 
 text \<open> Substitution update is idempotent. \<close>
@@ -156,13 +157,13 @@ lemma usubst_upd_var_id [usubst]:
 
 subsection \<open> Evaluation \<close>
 
-lemma subst_SEXP [usubst_eval]: "\<sigma> \<dagger> [\<lambda> s. e s]\<^sub>E = [\<lambda> s. e (\<sigma> s)]\<^sub>E"
+lemma subst_SEXP [usubst_eval]: "\<sigma> \<dagger> [\<lambda> s. e s]\<^sub>e = [\<lambda> s. e (\<sigma> s)]\<^sub>e"
   by (simp add: SEXP_def subst_app_def fun_eq_iff)
 
 lemma get_subst_id [usubst_eval]: "get\<^bsub>x\<^esub> (id\<^sub>s s) = get\<^bsub>x\<^esub> s"
   by (simp add: subst_id_def)
 
-lemma get_subst_upd_same [usubst_eval]: "weak_lens x \<Longrightarrow> get\<^bsub>x\<^esub> ((\<sigma>(x \<mapsto>\<^sub>s @e)) s) = e s"
+lemma get_subst_upd_same [usubst_eval]: "weak_lens x \<Longrightarrow> get\<^bsub>x\<^esub> ((\<sigma>(x \<mapsto>\<^sub>s e)) s) = e s"
   by (simp add: subst_upd_def SEXP_def)
 
 lemma get_subst_upd_indep [usubst_eval]: 
