Unrestriction.thy
@@ -9,17 +9,17 @@ syntax
   "_unrest" :: "salpha \<Rightarrow> logic \<Rightarrow> logic \<Rightarrow> logic" (infix "\<sharp>" 20)
 
 translations
-  "_unrest x p" == "CONST unrest x U(p)"                                           
+  "_unrest x p" == "CONST unrest x (p)\<^sub>e"                                           
   "_unrest (_salphaset (_salphamk (x +\<^sub>L y))) P"  <= "_unrest (x +\<^sub>L y) P"
 
 named_theorems unrest
 
 lemma unrest_var_comp [unrest]:
   "\<lbrakk> x \<sharp> P; y \<sharp> P \<rbrakk> \<Longrightarrow> x;y \<sharp> P"
-  by (simp add: expr_defs)
+  by (simp add: expr_defs lens_defs)
 
 lemma unrest_lens_comp [unrest]: "x \<sharp> e \<Longrightarrow> x:y \<sharp> e"
-  by (simp add: expr_defs)
+  by (simp add: expr_defs lens_defs)
 
 lemma unrest_lit [unrest]: "x \<sharp> \<guillemotleft>v\<guillemotright>"
   by (simp add: expr_defs)
@@ -29,15 +29,15 @@ lemma unrest_var [unrest]:
   by (simp add: expr_defs lens_indep.lens_put_irr2)
 
 lemma unrest_uop [unrest]:
-  "\<lbrakk> x \<sharp> @e \<rbrakk> \<Longrightarrow> x \<sharp> f (@e)"
+  "\<lbrakk> x \<sharp> e \<rbrakk> \<Longrightarrow> x \<sharp> \<guillemotleft>f\<guillemotright> e"
   by (auto simp add: expr_defs)
 
 lemma unrest_bop [unrest]:
-  "\<lbrakk> x \<sharp> @e\<^sub>1; x \<sharp> @e\<^sub>2 \<rbrakk> \<Longrightarrow> x \<sharp> f (@e\<^sub>1) (@e\<^sub>2)"
+  "\<lbrakk> x \<sharp> e\<^sub>1; x \<sharp> e\<^sub>2 \<rbrakk> \<Longrightarrow> x \<sharp> \<guillemotleft>f\<guillemotright> e\<^sub>1 e\<^sub>2"
   by (auto simp add: expr_defs)
 
 lemma unrest_trop [unrest]:
-  "\<lbrakk> x \<sharp> @e\<^sub>1; x \<sharp> @e\<^sub>2; x \<sharp> @e\<^sub>3 \<rbrakk> \<Longrightarrow> x \<sharp> f (@e\<^sub>1) (@e\<^sub>2) (@e\<^sub>3)"
+  "\<lbrakk> x \<sharp> e\<^sub>1; x \<sharp> e\<^sub>2; x \<sharp> e\<^sub>3 \<rbrakk> \<Longrightarrow> x \<sharp> \<guillemotleft>f\<guillemotright> e\<^sub>1 e\<^sub>2 e\<^sub>3"
   by (auto simp add: expr_defs)
 
 end
